Finished some of 3.1, formalized traces

scrap.v
@@ -4,83 +4,762 @@ From Coq Require Import Bool.Bool Init.Nat Arith.Arith Arith.EqNat
 Require Export Coq.Strings.String.
 From mathcomp Require Import ssreflect ssrfun ssrbool eqtype.
 Import ListNotations.
-From Semantics Require Export semantics.
+(*setting up*)
 Open Scope list_scope.
-(*relation determining what variables are read when evaluating exp e
+Fixpoint eq_lists {A: Type} (L1: list A) (L2: list A) (eq: A -> A -> Prop) :=
+        match L1, L2 with
+          nil, nil => True
+        | (w::ws), (d::ds) => (eq w d) /\ (eq_lists ws ds eq) (*considers order*)
+        | _ , _ => False end.
+
+Definition prefix {A: Type} (O1: list A) (O2: list A) :=
+  exists(l: nat), O1 = firstn l O2.
+
+Close Scope list_scope.
+
+Open Scope string_scope.
+Lemma eqnat: Equality.axiom Init.Nat.eqb.
+Proof.
+  unfold Equality.axiom. intros.
+  destruct (Init.Nat.eqb (x) (y)) eqn:beq.
+  - constructor. apply beq_nat_true in beq. assumption.
+  -  constructor. apply beq_nat_false in beq. assumption.
+Qed.
+Canonical nat_eqMixin := EqMixin eqnat.
+Canonical nat_eqtype := Eval hnf in EqType nat nat_eqMixin.
+(*---*)
+
+(*setting up strings equality type*)
+(* eqb_string and
+eqb_string_true_iff taken from software foundations*)
+Definition eqb_string (x y : string) : bool :=
+  if string_dec x y then true else false.
+
+Lemma eqb_string_true_iff : forall x y : string,
+    eqb_string x y = true <-> x = y.
+Proof.
+   intros x y.
+   unfold eqb_string.
+   destruct (string_dec x y) as [H |Hs].
+   - subst. split. reflexivity. reflexivity.
+   - split.
+     + intros contra. discriminate contra.
+     + intros H. rewrite H in Hs *. destruct Hs. reflexivity.
+Qed.
+(*what is the star*)
+Lemma eqstring: Equality.axiom eqb_string.
+Proof.
+  unfold Equality.axiom. intros.
+  destruct (eqb_string x y) eqn:beq.
+  - constructor. apply eqb_string_true_iff in beq. assumption.
+  -  constructor. intros contra. apply eqb_string_true_iff in contra.
+     rewrite contra in beq. discriminate beq.
+Qed.
+Canonical string_eqMixin := EqMixin eqstring.
+Canonical string_eqtype := Eval hnf in EqType string string_eqMixin.
+Close Scope string_scope.
+(***)
+
+
+(*Now, to business! Below is syntax*)
+Open Scope type_scope.
+
+Inductive boptype :=
+  Plus
+| Sub
+| Mult
+| Div
+| Mod
+| Or
+| And.
+
+(*shortcut!*)
+Inductive value :=
+    Nat (n: nat)
+  | Bool (b: bool)
+  | error. 
+Coercion Bool : bool >-> value.
+Coercion Nat : nat >-> value.
+
+(*evaluation rules for binary operations*)
+
+Fixpoint bopeval (bop: boptype) (v1 v2 :value): (value) :=
+  match bop with
+   Plus => 
+    (
+      match v1, v2 with
+        (Nat n1), (Nat n2) => Nat (add n1 n2)
+        | _, _ => error
+        end
+    )
+  | Sub => 
+    (
+      match v1, v2 with
+       (Nat n1), (Nat n2) => Nat (n1 - n2)
+        | _, _ => error
+        end
+    )
+  | Mult => 
+    (
+      match v1, v2 with
+       (Nat n1), (Nat n2) => Nat (mul n1 n2)
+        | _, _ => error
+        end
+    )
+  | Div =>
+    (
+      match v1, v2 with
+       (Nat n1), (Nat n2) =>
+                    ( if (n2 == 0) then error
+                      else Nat (n1 / n2))
+        | _, _ => error
+        end
+    )
+  | Mod =>
+    (
+      match v1, v2 with
+       (Nat n1), (Nat n2) =>
+                    ( if (n2 == 0) then error
+                     else Nat (n1 mod n2))
+        | _, _ => error
+        end
+    )
+  | Or =>
+  (
+      match v1, v2 with
+        (Bool b1), (Bool b2) => Bool (orb b1 b2)
+        | _, _ => error
+        end
+    )
+  | And =>
+  (
+      match v1, v2 with
+        (Bool b1), (Bool b2) => Bool (andb b1 b2)
+        | _, _ => error
+        end
+  )
+  end.
+
+(*value helper functions*)
+Definition isvaluable (v: value) :=
+  match v with
+    error => False
+  | _ => True
+  end.
+
+Definition isvalidbop (bop: boptype) (v1 v2 : value) :=
+  match (bopeval bop v1 v2) with
+    error => False
+  | _ => True
+   end.
+
+Definition eqb_value (x y: value) :=
+  match x, y with
+    Nat nx, Nat ny => nx == ny
+  | Bool bx, Bool byy => eqb bx byy
+  | _, _ => false
+  end.
+Definition eq_value (x y: value) := is_true(eqb_value x y).
+
+Definition eq_valueop (x y : option value) :=
+  match x, y with
+    Error, None => True
+  | Some x1, Some y1 => eq_value x1 y1
+  | _, _ => False
+  end.
+
+(*memory maps...used for both memories and checkpoints*)
+Definition map (A: Type) (eqba: A -> A -> bool):= A -> value.
+
+(*memory helpers*)
+Definition emptymap A eqba :(map A eqba) := (fun _ => error).
+Definition updatemap {A} {eqba} (m: map A eqba) (i: A) (v: value) : map A eqba := (fun j =>
+                                                               if (eqba j i) then v
+                                                               else (m j)).
+Notation "i '|->' v ';' m" := (updatemap m i v)
+  (at level 100, v at next level, right associativity).
+(*in (m1 U! m2), m1 is checked first, then m2*)
+
+Definition indomain {A} {eqba} (m: map A eqba) (x: A) :=
+  match m x with
+    error => False
+  | _ => True
+  end.
+(*this function is NOT used to check the domain of checkpoint maps.
+ In particular, because an entire array can be checkpointed even if only
+ one element has been assigned to (while the other elements may, in theory, still be unassigned),
+(in particular, I refer to D-WAR-CP-Arr)
+this function would return that assigned array elements are in the domain of N, while the unassigned array
+elements are not, even though both have been checkpointed.
+ I resolved this problem by defining indomain_nvm, used for checkpoint maps in algorithms.v, which
+checks if a warvar is in the domain, rather than checking a location.
  *)
-(*N, V are dummy values*)
-Inductive rd: exp -> warvars -> Prop :=
-    RD (e: exp) (N: nvmem) (V: vmem) (rs: readobs) (v: value):
-      eeval N V e rs v -> rd e (readobs_warvars rs).
+(******************************************************************************************)
 
-Inductive warcheck: nvmem -> warvars -> warvars -> instruction -> warvars -> warvars -> Prop := 
-  WAR_Skip: forall(N: nvmem) (W: warvars) (R: warvars),
-    warcheck N W R skip W R
-| WAR_NoRd: forall(N: nvmem) (W: warvars) (R: warvars)
-             (x: smallvar) (e: exp)
-             (Re: warvars),
-             (rd e Re) -> (*extra premise checking that Re is the list of values read when e is evaluated*)
-             not(memberwv_wv (inl x) (R ++ Re)) 
-             -> warcheck N W R (asgn_sv x e) ((inl x)::W) (R ++ Re)
-| WAR_Checkpointed: forall(N: nvmem) (W: warvars) (R: warvars)
-             (x: smallvar) (e: exp)
-             (Re: warvars),
-             (rd e Re) -> (*extra premise checking that Re is the list of values read when e is evaluated*)
-             memberwv_wv (inl x) (R ++ Re) ->
-             not(memberwv_wv (inl x) W) ->
-             (indomain_nvm N (inl x)) ->
-             warcheck N W R (asgn_sv x e) ((inl x)::W) (R ++ Re)
-| WAR_WT: forall(N: nvmem) (W: warvars) (R: warvars)
-             (x: smallvar) (e: exp)
-             (Re: warvars),
-             (rd e Re) -> (*extra premise checking that Re is the list of values read when e is evaluated*)
-             memberwv_wv (inl x) (R ++ Re) ->
-             (memberwv_wv (inl x) W) ->
-             warcheck N W R (asgn_sv x e) W (R ++ Re)
-| WAR_NoRd_Arr: forall(N: nvmem) (W: warvars) (R: warvars)
-                 (a: array) (index: exp) (Rindex: warvars)
-                 (e: exp) (Re: warvars),
-    (rd e Re) -> (*extra premise checking that Re is the list of values read when e is evaluated*)
-    (rd index Rindex) -> (*extra premise checking that Rindex is the list of values read when index is evaluated*)
-    not(memberwv_wv (inr a) (R ++ Re ++ Rindex)) ->
-    warcheck N W R (asgn_arr a index e) ((inr a)::W) (R ++ Re ++ Rindex)
-| WAR_Checkpointed_Arr: forall(N: nvmem) (W: warvars) (R: warvars)
-                 (a: array) (index: exp) (Rindex: warvars)
-                 (e: exp) (Re: warvars),
-    (rd e Re) -> (*extra premise checking that Re is the list of values read when e is evaluated*)
-    (rd index Rindex) -> (*extra premise checking that Rindex is the list of values read when index is evaluated*)
-    (memberwv_wv (inr a) (R ++ Re ++ Rindex)) ->
-    (indomain_nvm N (inr a)) ->
-    warcheck N W R (asgn_arr a index e) ((inr a)::W) (R ++ Re ++ Rindex)
-.
-(*Inductive warcheck: nvmem -> warvars -> warvars -> instruction -> warvars -> warvars -> Prop := *)
-Inductive WARok: nvmem -> warvars -> warvars -> command -> Prop:=
-  WAR_I: forall(N: nvmem) (W: warvars) (R: warvars) (l: instruction)
-          (W': warvars) (R': warvars),
-    warcheck N W R l W' R' -> WARok N W R l
- | WAR_CP: forall(w: warvars) (c: command)
-            (N N': nvmem) (*N' is the checkpoint memory map*)
-            (W: warvars) (R: warvars),
-     (isdomain_nvm N' w) -> (*extra premise checking that N' does map exactly the things in w*)
-       WARok N' nil nil c ->
-       WARok N W R ((incheckpoint w);;c)
- | WAR_Seq: forall(N: nvmem) (W W' R R': warvars)
-             (l: instruction) (c: command),
-             warcheck N W R l W' R' ->
-             WARok N W' R' c ->
-             WARok N W R (l;;c)
- | WAR_If: forall(N: nvmem)
-            (W R Re: warvars)
-            (e: exp)
-            (c1 c2: command),
-     (rd e Re) -> (*extra premise checking that Re is the list of values read when e is evaluated*)
-     WARok N W (R ++ Re) c1 ->
-     WARok N W (R ++ Re) c2 ->
-     WARok N W R (TEST e THEN c1 ELSE c2)
+(*******************************more syntax**********************************************)
+Inductive array :=
+  Array (s: string) (l: nat).
+
+
+Inductive volatility :=
+  nonvol
+ | vol.
+
+Inductive exp :=
+  Var (s: string) (q: volatility) 
+| Val (v: value)
+| Bop (bop: boptype) (e1: exp) (e2: exp) 
+| El (a: array) (e: exp).
+Coercion Val : value >-> exp.
+Notation "a '[[' e ']]'" := (El (a) (e))
+                            (at level 100, right associativity).
+(*used subtypes to enforce the fact that only some expressions are
+ memory locations*)
+(*also made the write after read type easier*)
+Definition smallvarpred := (fun x=> match x with
+                                        Var _ _ => true
+                                        | _ => false
+                                 end).
+Definition elpred  := (fun x=> match x with
+                                        El (Array _ length) (Val (Nat i)) => (i <? length)
+                                        | _ => false
+                                 end).
+(*note elpred checks if index is a natural in bounds*)
+Notation smallvar := {x: exp | smallvarpred x}.
+Notation el := {x: exp| elpred x}.
+Definition loc := smallvar + el. (*memory location type*)
+
+Definition warvar := smallvar + array. (*write after read variable type*)
+Notation warvars := (list warvar).
+(*Coercion (inl smallvar el): smallvar >-> loc.*)
+(*Coercion inl: smallvar >-> loc.*)
+
+(**location and warvar helper functions*)
+(**no need to work directly with the subtypes or sumtypes, just use these**)
+(**Note: some of these are currently unused due to implementation changes, but I left them
+ as they might be useful later*)
+
+(*array and el functions*)
+
+(*checks name and length*)
+Open Scope list_scope.
+Definition eqb_array (a1 a2: array) :=
+  match a1, a2 with
+    Array s1 l1, Array s2 l2 => andb (s1 == s2) (l1 == l2)
+    end.
+Program Definition getarray (x: el): array :=
+  match val x with
+    El (arr) _ => arr
+  | _ => !
+  end.
+Next Obligation. destruct (x) as [s| | |];
+                 try (simpl in H0; discriminate H0).
+     apply (H a e). reflexivity.
+Qed.
+
+Program Definition getindexel (x: el): value  :=
+  match val x with
+    El _ (Val v) => v
+  | _ => !
+  end.
+Next Obligation. destruct (x) as [s| | |];
+                 try (simpl in H0; discriminate H0).
+                 destruct a eqn: adestruct.
+                 destruct e;
+                 try (simpl in H0; discriminate H0).
+                 apply (H a v). subst. reflexivity.
+Qed.
+
+Definition samearray_b (element: el) (a: array) := (*checks if element indexes into a*)
+  eqb_array (getarray element) a.
+
+Definition samearray (element: el) (a: array) := is_true(samearray_b element a).
+
+Definition el_arrayind_eq (e: el) (a: array) (vindex: value) := (*transitions from el type
+                                                          to a[i] representation*)
+  (samearray e a) /\ (eq_value (getindexel e) vindex).
+
+(*smallvar functions*)
+Definition isNV_b (x: smallvar) := (*checks if x is stored in nonvolatile memory*)
+  match (val x) with
+    Var _ nonvol => true
+  | _ => false
+  end.
+
+Definition isV_b (x: smallvar) :=(*checks if x is stored in volatile memory*)
+  match (val x) with
+    Var _ vol => true
+  | _ => false
+  end.
+
+Definition isNV x := is_true(isNV_b x). (*prop version of isNV_b*)
+
+Definition isV x := is_true(isV_b x). (*prop version of isV_b*)
+
+Definition samevolatility_b (x y: smallvar) := (*used for defining equality of memory locations*)
+  match isNV_b(x), isNV_b(y) with
+    true, true => true
+  | false, false => true
+  | _, _ => false
+  end.
+
+Program Definition getstringsv (x: smallvar): string :=
+  match val x with
+    Var s _ => s
+  | _ => !
+  end. 
+Next Obligation.
+    destruct x as [s| | |];
+      try (simpl in H0; discriminate H0). apply (H s q). reflexivity.
+Qed.
+
+Definition eqb_smallvar (x y: smallvar): bool :=
+  andb ((getstringsv x)==(getstringsv y)) (samevolatility_b x y).
+
+(*loc and warvar functions*)
+Definition eqb_warvar (w1 w2: warvar) :=
+  match w1, w2 with
+               inl x, inl y => eqb_smallvar x y
+             | inr x, inr y => eqb_array x y
+             | _, _ => false
+  end.
+
+Definition eq_warvar (w1 w2: warvar) :=
+  is_true (eqb_warvar w1 w2).
+
+(*checks if w was recorded as read/written to in warvar list W*)
+Fixpoint memberwv_wv_b (input: warvar) (w: warvars) :=
+  match w with
+    [] => false
+  | wv::wvs => orb (eqb_warvar input wv) (memberwv_wv_b input wvs) 
+end.
+
+Definition memberwv_wv (w: warvar) (W: warvars) := is_true(memberwv_wv_b w W).
+
+
+Definition eqb_loc (l1: loc) (l2: loc) :=
+  match l1, l2 with
+    inl x, inl y => eqb_smallvar x y
+  | inr x, inr y => andb (eqb_array (getarray x) (getarray y))
+                        (eqb_value (getindexel x) (getindexel y))
+  | _, _ => false 
+  end. (*might be nice to have values as an equality type here*)
+
+(*converts a location to a warvar*)
+Fixpoint loc_warvar (l: loc) : warvar := 
+  match l with
+    inl x => inl x
+  | inr el => inr (getarray el)
+  end.
+
+(*checks if a location input has been stored as a WAR location in w*)
+Definition memberloc_wvs_b (input: loc) (w: warvars) :=
+  memberwv_wv_b (loc_warvar input) w.
+(*******************************************************************)
+
+(*more syntax*)
+Inductive instruction :=
+  skip
+| asgn_sv (x: smallvar) (e: exp) (*could distinguish between NV and V assignments as well here*)
+| asgn_arr (a: array) (i: exp) (e: exp) (*i is index, e is new value of a[i]*)
+| incheckpoint (w: warvars)
+| inreboot.
+(*added the in prefixes to distinguish from the observation reboots
+ and checkpoints*)
+
+Inductive command :=
+  Instruct (l: instruction)
+| Seqcom (l: instruction) (c: command) (*added suffix to distinguish from Seq ceval
+                                         constructor*)
+| ite (e: exp) (c1: command) (c2: command).
+
+Notation "l ';;' c" := (Seqcom l c)
+                         (at level 100).
+
+Notation "'TEST' e 'THEN' c1 'ELSE' c2 " := (ite e c1 c2)
+                                              (at level 100).
+Coercion Instruct : instruction >-> command.
+(*******************************************************************)
+
+(******setting up location equality relation for memory maps******************)
+(****************************************************************)
+
+(****************************memory*************************************)
+
+(*memory locations defined above warvars*)
+Notation mem := (map loc eqb_loc). (*memory mapping*)
+
+Inductive nvmem := (*nonvolatile memory*)
+  NonVol (m : mem) (D: warvars). (*extra argument to keep track of checkpointed warvars because
+                                  it might be nice to have for when we do checkpoint proofs*)
+
+Inductive vmem := (*volatile memory*)
+  Vol (m : mem).
+
+(*I could change nvmem and vmem to enforce that they only take in smallvars
+ of the correct type but it's already checked in my evaluation rules*)
+
+(**************************helpers for the memory maps*********************************************)
+
+(*note: a lot of these aren't being used right now because, after I changed the types
+ of DINO and WAR, they aren't necessary.
+ I won't delete them because having the domain of the checkpoint easily accessible and
+ manipulable could be handy in the future*)
+
+Definition getmap (N: nvmem) :=
+  match N with NonVol m _ => m end.
+
+Definition getdomain (N: nvmem) :=
+  match N with NonVol _ D => D end.
+
+Definition getvalue (N: nvmem) (i: loc) :=
+  (getmap N) i.
+  Notation "v '<-' N" := (getvalue N v)
+                           (at level 40).
+
+
+  (*updates domain and mapping function*)
+Definition updateNV (N: nvmem) (i: loc) (v: value) :=
+  match N with NonVol m D =>
+               NonVol (updatemap m i v) (
+                        match i with 
+                          inl x => ((inl x) :: D) (*i is a smallvar*)
+                        | inr el => ((inr (getarray el))::D) (*i is an array element*)
+                                     (*here I add the entire array to the domain
+                                      even though only one element has been assigned to*)
+                        end
+                      )
+  end.
+
+(*used to update NV memory with checkpoint*)
+(*checks N first, then N'*)
+Definition updatemaps (N: nvmem) (N': nvmem): nvmem :=
+  match N, N' with
+    NonVol m D, NonVol m' D' => NonVol
+  (fun j =>
+     match m j with
+     error => m' j
+     | x => x
+     end
+  )
+  (D ++ D') (*inclusion of duplicates*)
+  end.
+Notation "m1 'U!' m2" := (updatemaps m1 m2) (at level 100).
+
+Notation emptyNV := (NonVol (emptymap loc eqb_loc) nil).
+Definition reset (V: vmem) := Vol (emptymap loc eqb_loc).
+
+(*restricts memory map m to domain w*)
+(*doesn't actually clean the unnecessary variables out of m*)
+Definition restrict (N: nvmem) (w: warvars): nvmem :=
+  match N with NonVol m D => NonVol
+    (fun input => if (memberloc_wvs_b input w) then m input else error) w  end.
+
+Notation "N '|!' w" := (restrict N w) 
+  (at level 40, left associativity).
+
+(*prop determining if every location in array a is in the domain of m*)
+Definition indomain_nvm (N: nvmem) (w: warvar) :=
+  memberwv_wv_b w (getdomain N).
+
+Definition isdomain_nvm (N: nvmem) (w: warvars) :=
+  eq_lists (getdomain N) w eq_warvar.
+
+(********************************************)
+Inductive cconf := (*continuous configuration*)
+  ContinuousConf (triple: nvmem * vmem * command).
+
+Notation context := (nvmem * vmem * command). 
+
+Inductive iconf := (*intermittent configuration*)
+  IntermittentConf (qple: context * nvmem * vmem * command).
+
+Definition ro := loc * value. (*read observation*)
+Definition readobs := list ro.
+
+Notation NoObs := ([]: readobs).
+
+Inductive obs := (*observation*)
+  Obs (r: readobs)
+| reboot
+| checkpoint.
+Coercion Obs : readobs >-> obs.
+
+Notation obseq := (list obs). (*observation sequence*)
+
+Open Scope list_scope.
+
+(*helpers for observations and warvars*)
+(*don't need the first two as there's no way to construct
+ a relation instance that would violate these*)
+Definition hasCheckpt (O: obseq) := In checkpoint O.
+
+Definition isAllRead (O: obseq) := not(hasCheckpt O) /\ not(In reboot O).
+
+(*converts from list of read locations to list of
+WAR variables
+ *)
+Fixpoint readobs_warvars (R: readobs) : warvars := 
+  match R with
+    nil => nil
+| (r::rs) => match r with
+              (location, _) => (*get the location r has recorded reading from*)
+              (match location with
+                inl x => (inl x)::(readobs_warvars rs) (*location is a smallvar*)
+              | inr el => (inr (getarray el))::(readobs_warvars rs) (*location is an array element
+                                                                   records entire array in warvars*)
+              end)
+           end
+  end.
+
+(*relations between continuous and intermittent traces*)
+(*Definition reduces (O1 O2: readobs) :=
+  (prefix O1 O2*)
+Notation "S <= T" := (prefix S T).
+
+(*Where
+O1 is a sequence of read observation lists,
+where each continguous read observation list is separated from those adjacent to it by a reboot,
+and O2 is a read observation list,
+prefix_seq determines if each ro list in O1 is a valid
+prefix of O2*)
+Inductive prefix_seq: obseq -> readobs -> Prop :=
+  RB_Base: forall(O: readobs), prefix_seq [Obs O] O
+| RB_Ind: forall(O1 O2: readobs) (O1': obseq),
+    O1 <= O2 -> prefix_seq O1' O2 -> prefix_seq ([Obs O1] ++ [reboot] ++ O1') O2.
+
+(* Where
+O1 is a sequence of ((read observation list sequences), where
+each continguous read observation list is separated from those adjacent to it
+by a reboot), where each sequence is separated from those adjacent to it by a checkpoint.
+ie, each read observation list in a given read observation sequence
+occurs within the same checkpointed region as all the other read observation lists in that sequence,
+O2 is a read observation list,
+prefix_frag determines if each ro list in O1 is a prefix of some FRAGMENT of O2
+(where the fragments are separated by the positioning of the checkpoints in O1)
+ *)
+Inductive prefix_fragment: obseq -> readobs -> Prop :=
+  CP_Base: forall(O1: obseq) (O2: readobs), prefix_seq O1 O2 -> prefix_fragment O1 O2
+| CP_IND: forall(O1 O1': obseq) (O2 O2': readobs),
+    prefix_seq O1 O2 -> prefix_fragment O1' O2' ->
+   prefix_fragment (O1 ++ [checkpoint] ++ O1') (O2 ++ O2'). 
+
+(***************************************************************)
+
+(*traces*)
+(*The trace type contains
+1. a list of configurations, where each configuration follows from
+ its leftmost neighbor by an evaluation rule
+2. a list of warvars which have been written to
+3. a list of warvars which have been read from
+4. a list of warvars which have been written to before they have been read from
+ *)
+
+Inductive trace_c: list cconf -> warvars -> warvars -> warvars -> Prop :=
+  Empty: trace_c nil nil nil nil
+| 
 .
 
-Inductive DINO: nvmem -> warvars -> warvars -> instruction
-                -> nvmem -> warvars -> warvars Prop:=
-  D_ WAR_Skip: forall(N: nvmem) (W: warvars) (R: warvars)
-          (W': warvars) (R': warvars),
-    warcheck N W R l W' R' -> WARok N W R l
+    (*need starting point and ending point for trace*)
+
+(****************continuous operational semantics***********************)
+(*evaluation relation for expressions*)
+Inductive eeval: nvmem -> vmem -> exp -> readobs -> value -> Prop :=
+  VAL: forall(N: nvmem) (V: vmem) (v: value),
+    (isvaluable v) -> (*extra premise to check if v is valuable*)
+    eeval N V v NoObs v
+| BINOP: forall(N: nvmem) (V: vmem)
+          (e1: exp) (e2: exp)
+          (r1: readobs) (r2: readobs)
+          (v1: value) (v2: value) (bop: boptype),
+    eeval N V e1 r1 v1 ->
+    eeval N V e2 r2 v2 -> 
+    (isvalidbop bop v1 v2) -> (*extra premise to check if v1, v2, bop v1 v2 valuable*)
+    eeval N V (Bop bop e1 e2) (r1++ r2) (bopeval bop v1 v2)
+| RD_VAR_NV: forall(N: nvmem) (mapV: vmem) (x: smallvar) (v: value),
+    eq_value ((inl x) <-N) v ->
+    isNV(x) -> (*extra premise to make sure x is correct type for NV memory*)
+    (isvaluable v) -> (*extra premise to check if v is valuable*)
+    eeval N mapV (val x) [((inl x), v)] v
+| RD_VAR_V: forall(N: nvmem) (mapV: mem) (x: smallvar) (v: value),
+    eq_value (mapV (inl x)) v ->
+    isV(x) -> (*extra premise to make sure x is correct type for V memory*)
+    (isvaluable v) -> (*extra premise to check if v is valuable*)
+    eeval N (Vol mapV) (val x) [((inl x), v)] v
+| RD_ARR: forall(N: nvmem) (V: vmem)
+           (a: array)
+           (index: exp)
+           (rindex: readobs)
+           (vindex: value)
+           (element: el)
+           (v: value),
+    eeval N V (index) rindex vindex ->
+    eq_value ((inr element) <-N) v ->
+    (el_arrayind_eq element a vindex) -> (*extra premise to check that inr element
+                                        is actually a[vindex] *)
+(*well-typedness, valuability, inboundedness of vindex are checked in elpred*)
+    (isvaluable v) -> (*extra premise to check if v is valuable*)
+    eeval N V (a[[index]]) (rindex++[((inr element), v)]) v
+.
+(*ask Arthur why this notation doesn't work *)
+
+(*Reserved Notation "'{'N V'}=[' e ']=> <'r'>' v" (at level 40).
+Inductive eevaltest: nvmem -> vmem -> exp -> obs -> value -> Prop :=
+  VAL: forall(N: nvmem) (V: vmem) (v: value), 
+    {N V} =[ v ]=> <reboot> v
+  where "{N V}=[ e ]=> <r> v" := (eevaltest N V e r v).*)
+
+(****************************************************************************)
+
+(**********continuous execution semantics*************************)
+
+
+(*evaluation relation for commands*)
+Inductive cceval: nvmem -> vmem -> command -> obseq -> nvmem -> vmem -> command -> Prop :=
+  NV_Assign: forall(x: smallvar) (N: nvmem) (V: vmem) (e: exp) (r: readobs) (v: value),
+    eeval N V e r v ->
+    isNV(x) -> (*checks x is correct type for NV memory*)
+    (isvaluable v) -> (*extra premise to check if v is valuable*)
+    cceval N V (asgn_sv x e) [Obs r]
+           (updateNV N (inl x) v) V skip
+| V_Assign: forall(x: smallvar) (N: nvmem) (mapV: mem) (e: exp) (r: readobs) (v: value),
+    eeval N (Vol mapV) e r v ->
+    isV(x) -> (*checks x is correct type for V memory*)
+    (isvaluable v) -> (*extra premise to check if v is valuable*)
+    cceval N (Vol mapV) (asgn_sv x e) [Obs r] N (Vol ((inl x) |-> v ; mapV)) skip
+| Assign_Arr: forall (N: nvmem) (V: vmem)
+               (a: array)
+               (ei: exp)
+               (ri: readobs)
+               (vi: value)
+               (e: exp)
+               (r: readobs)
+               (v: value)
+               (element: el),
+    eeval N V ei ri vi ->
+    eeval N V e r v ->
+    (el_arrayind_eq element a vi) -> (*extra premise to check that inr element
+                                        is actually a[vindex] *)
+(*well-typedness, valuability, inboundedness of vindex are checked in elpred*)
+    (isvaluable v) -> (*extra premise to check if v is valuable*)
+    cceval N V (asgn_arr a ei e) [Obs (ri++r)]
+           (updateNV N (inr element) v) V skip
+    (*valuability and inboundedness of vindex are checked in sameindex*)
+| CheckPoint: forall(N: nvmem)
+               (V: vmem)
+               (c: command)
+               (w: warvars),
+               cceval N V ((incheckpoint w);; c) [checkpoint]
+               N V c
+| Skip: forall(N: nvmem)
+         (V: vmem)
+         (c: command),
+    cceval N V (skip;;c) [Obs NoObs] N V c
+| Seq: forall (N: nvmem)
+         (N': nvmem)
+         (V: vmem)
+         (V': vmem)
+         (l: instruction)
+         (c: command)
+         (o: obs),
+    cceval N V l [o] N' V' skip ->
+    cceval N V (l;;c) [o] N' V' c
+| If_T: forall(N: nvmem)
+         (V: vmem)
+         (e: exp)
+         (r: readobs)
+         (c1: command)
+         (c2: command),
+    eeval N V e r true -> 
+    cceval N V (TEST e THEN c1 ELSE c2) [Obs r] N V c1
+| If_F: forall(N: nvmem)
+         (V: vmem)
+         (e: exp)
+         (r: readobs)
+         (c1: command)
+         (c2: command),
+    eeval N V e r false ->
+    cceval N V (TEST e THEN c1 ELSE c2) [Obs r] N V c2.
+
+(************************************************************)
+
+(**********intermittent execution semantics*************************)
+(*evaluation relation for commands*)
+Inductive iceval: context-> nvmem -> vmem -> command -> obseq -> context -> nvmem -> vmem -> command -> Prop :=
+  CP_PowerFail: forall(k: context) (N: nvmem) (V: vmem) (c: command),
+                 iceval k N V c
+                        [Obs NoObs]
+                        k N (reset V) inreboot
+ | CP_CheckPoint: forall(k: context) (N: nvmem) (V: vmem) (c: command) (w: warvars),
+                 iceval k N V ((incheckpoint w);;c)
+                        [checkpoint]
+                        ((N |! w), V, c) N V c 
+ | CP_Reboot: forall(N: nvmem) (N': nvmem)(*see below*) (*N is the checkpointed one*)
+               (V: vmem) (V': vmem)
+               (c: command), 
+     iceval (N, V, c) N' V' inreboot
+            [reboot]
+            (N, V, c) (N U! N') V c
+ | CP_NV_Assign: forall(k: context) (x: smallvar) (N: nvmem) (V: vmem) (e: exp) (r: readobs) (v: value),
+    eeval N V e r v ->
+    isNV(x) -> (*checks x is correct type for NV memory*)
+    (isvaluable v) -> (*extra premise to check if v is valuable*)
+    iceval k N V (asgn_sv x e)
+           [Obs r]
+           k (updateNV N (inl x) v) V skip
+| CP_V_Assign: forall(k: context) (x: smallvar) (N: nvmem) (mapV: mem) (e: exp) (r: readobs) (v: value),
+    eeval N (Vol mapV) e r v ->
+    isV(x) -> (*checks x is correct type for V memory*)
+    (isvaluable v) -> (*extra premise to check if v is valuable*)
+    iceval k N (Vol mapV) (asgn_sv x e)
+           [Obs r]
+           k N (Vol ((inl x) |-> v ; mapV)) skip
+| CP_Assign_Arr: forall (k: context) (N: nvmem) (V: vmem)
+               (a: array)
+               (ei: exp)
+               (ri: readobs)
+               (vi: value)
+               (e: exp)
+               (r: readobs)
+               (v: value)
+               (element: el),
+    eeval N V ei ri vi ->
+    eeval N V e r v ->
+    (el_arrayind_eq element a vi) -> (*extra premise to check that inr element
+                                        is actually a[vindex] *)
+(*well-typedness, valuability, inboundedness of vindex are checked in elpred*)
+    (isvaluable v) -> (*extra premise to check if v is valuable*)
+    iceval k N V (asgn_arr a ei e)
+           [Obs (ri++r)]
+           k (updateNV N (inr element) v) V skip
+| CP_Skip: forall(k: context) (N: nvmem)
+         (V: vmem)
+         (c: command),
+    iceval k N V (skip;;c) [Obs NoObs] k N V c
+|CP_Seq: forall (k: context)
+         (N: nvmem) (N': nvmem)
+         (V: vmem) (V': vmem)
+         (l: instruction)
+         (c: command)
+         (o: obs),
+    iceval k N V l [o] k N' V' skip ->
+    iceval k N V (l;;c) [o] k N' V' c
+|CP_If_T: forall(k: context) (N: nvmem) (V: vmem)
+         (e: exp)
+         (r: readobs)
+         (c1: command)
+         (c2: command),
+    eeval N V e r true -> 
+    iceval k N V (TEST e THEN c1 ELSE c2) [Obs r] k N V c1
+|CP_If_F: forall(k: context) (N: nvmem) (V: vmem)
+         (e: exp)
+         (r: readobs)
+         (c1: command)
+         (c2: command),
+    eeval N V e r false ->
+    iceval k N V (TEST e THEN c1 ELSE c2) [Obs r] k N V c2.
+(*CP_Reboot: I took out the equals premise and instead built it
+into the types because I didn't want to define a context equality function*)
+
+Close Scope list_scope.
+Close Scope type_scope.
